src/WeierstrassCurve/Pre.v
@@ -9,13 +9,16 @@ Local Open Scope core_scope.
 
 Generalizable All Variables.
 Section Pre.
-  Context {F eq zero one opp add sub mul inv div} {field:@field F eq zero one opp add sub mul inv div} {eq_dec: DecidableRel eq} {char_gt_2:@Ring.char_gt F eq zero one opp add sub mul 2%N}.
-  Local Infix "=" := eq. Local Notation "a <> b" := (not (a = b)).
-  Local Infix "=" := eq : type_scope. Local Notation "a <> b" := (not (a = b)) : type_scope.
-  Local Notation "0" := zero.  Local Notation "1" := one.
-  Local Infix "+" := add. Local Infix "*" := mul.
-  Local Infix "-" := sub. Local Infix "/" := div.
-  Local Notation "- x" := (opp x).
+  Context {F Feq Fzero Fone Fopp Fadd Fsub Fmul Finv Fdiv}
+          {field:@field F Feq Fzero Fone Fopp Fadd Fsub Fmul Finv Fdiv}
+          {char_gt_2:@Ring.char_gt F Feq Fzero Fone Fopp Fadd Fsub Fmul 2%N}
+          {eq_dec: DecidableRel Feq}.
+  Local Infix "=" := Feq. Local Notation "a <> b" := (not (a = b)).
+  Local Infix "=" := Feq : type_scope. Local Notation "a <> b" := (not (a = b)) : type_scope.
+  Local Notation "0" := Fzero.  Local Notation "1" := Fone.
+  Local Infix "+" := Fadd. Local Infix "*" := Fmul.
+  Local Infix "-" := Fsub. Local Infix "/" := Fdiv.
+  Local Notation "- x" := (Fopp x).
   Local Notation "x ^ 2" := (x*x). Local Notation "x ^ 3" := (x*x^2).
   Local Notation "'∞'" := unit : type_scope.
   Local Notation "'∞'" := (inr tt) : core_scope.
@@ -26,31 +29,34 @@ Section Pre.
   Context {b:F}.
 
   (* the canonical definitions are in Spec *)
-  Definition onCurve (P:F*F + ∞) := match P with
-                                    | (x, y) => y^2 = x^3 + a*x + b
-                                    | ∞ => True
-                                    end.
-  Definition unifiedAdd' (P1' P2':F*F + ∞) : F*F + ∞ :=
-    match P1', P2' with
-    | (x1, y1), (x2, y2)
-      => if dec (x1 = x2) then
-           if dec (y2 = -y1) then
-             ∞
-           else ((3*x1^2+a)^2 / (2*y1)^2 - x1 - x1,
-                   (2*x1+x1)*(3*x1^2+a) / (2*y1) - (3*x1^2+a)^3/(2*y1)^3-y1)
-         else
-           ((y2-y1)^2 / (x2-x1)^2 - x1 - x2,
-            (2*x1+x2)*(y2-y1) / (x2-x1) - (y2-y1)^3 / (x2-x1)^3 - y1)
+  Let onCurve (P:F*F + ∞) := match P with
+                             | (x, y) => y^2 = x^3 + a*x + b
+                             | ∞ => True
+                             end.
+  Let add (P1' P2':F*F + ∞) : F*F + ∞ :=
+    match P1', P2' return _ with
+    | (x1, y1), (x2, y2) =>
+      if dec (x1 = x2)
+      then
+        if dec (y2 = -y1)
+        then ∞
+        else let k := (3*x1^2+a)/(2*y1) in
+             let x3 := k^2-x1-x1 in
+             let y3 := k*(x1-x3)-y1 in
+             (x3, y3)
+      else let k := (y2-y1)/(x2-x1) in
+           let x3 := k^2-x1-x2 in
+           let y3 := k*(x1-x3)-y1 in
+           (x3, y3)
     | ∞, ∞ => ∞
     | ∞, _ => P2'
     | _, ∞ => P1'
     end.
 
-  Lemma unifiedAdd'_onCurve P1 P2 
-    (O1:onCurve P1) (O2:onCurve P2) : onCurve (unifiedAdd' P1 P2).
+  Lemma add_onCurve P1 P2 (_:onCurve P1) (_:onCurve P2) :
+    onCurve (add P1 P2).
   Proof.
     destruct_head' sum; destruct_head' prod;
-      cbv [onCurve unifiedAdd'] in *; break_match;
-        trivial; [|]; setoid_subst_rel eq; fsatz.
+      cbv [onCurve add] in *; break_match; trivial; [|]; fsatz.
   Qed.
 End Pre.
